mapAccum and mapKeys functions

examples/containers/theories/MapProofs/MapFunctionProofs.v
@@ -8,35 +8,30 @@ Require Import Psatz.
 Require Import Tactics.
 Set Bullet Behavior "Strict Subproofs".
 Require Import MapProofs.Bounds.
+Require Import MapProofs.Tactics.
 Require Import MapProofs.ContainerAxiomsProofs.
 Require Import MapProofs.UnionIntersectDifferenceProofs.
-(** ** Verification of [map] *)
+Require Import MapProofs.ToListProofs.
+Require Import MapProofs.FilterPartitionProofs.
+Require Import MapProofs.FromListProofs.
+Require Import Coq.Classes.Morphisms.
+(** ** Verification of [mapWithKey] *)
 
-(*Note: for map_spec, the definition we want is not provable:
-[(forall i v, sem m i = Some v <-> sem (mapWithKey f m) i = Some (f i v))]
+Lemma mapWithKey_Desc: forall {e} {a} {b} `{OrdLaws e} (m: Map e a) (f: e -> a -> b) lb ub,
+  Bounded m lb ub ->
+  Proper ((fun i j : e => _GHC.Base.==_ i j = true) ==> eq) f ->
+  Desc (mapWithKey f m) lb ub (size m) (fun i => match (sem m i) with
+                                                 | Some x => Some (f i x)
+                                                 | None => None end).
+Proof.
+  intros. induction H0.
+  - simpl. solve_Desc e.
+  - simpl. applyDesc e IHBounded1. applyDesc e IHBounded2. solve_Desc e. f_solver e.
+    assert (f x v = f i v). apply equal_f. apply H1. order e. rewrite H5. reflexivity.
+Qed.
 
-This is because of three problems
-1. Even if two keys k1 and k2 are equal (k1 == k2), this does not guarantee
-   that (f k = f k2).
-2. We cannot compare the results using Haskell equality because neither a not b
-   are required to be members of Eq.
-3. If f is not injective, then the (<-) is clearly not true (for example, 
-   suppose f = \x -> \y -> 1)
-
-This is not an issue in SetProofs because [Ord b] is a necessary condition for the input and the
-map function is defined very differently, leading to an entirely different specification.
-
-There are two solutions to this: 
-1. Require that if k == k1 and v == v1, then f k v = f k1 v1, which is not true in general
-2. Require that [a] and [b] be members of [Eq], which is also not true in general. We also must
-   require that k1 == k2 and v1 == v2 -> f k1 v1 == f k2 v2, which should be true in all cases, since
-   this is the definition of a pure function in Haskell.
-
-Both cases are proved below. We prove both cases because it could happen that Haskell equality agrees
-with Coq equality on the values but the values are not an instance of [Ord] (and this will be used in
-[FMapInterface]
-
-*)
+(*The following are several other lemmas about [map] and [mapWithKey] that are useful
+for [FMapInterface]*)
 
 (*Specification using Coq equality*)
 
@@ -61,9 +56,9 @@ Qed.
 (*Says that if we take any (key, value) pair in the map resulting from mapWithKey, then they
 come from a corresponding entry in the original map*)
 Lemma map_spec_reverse : 
-  forall {b} {a} {t}  `{Ord t} (H : EqLaws t) (f : t -> a -> b) (m : Map t a) lb ub,
+  forall {b} {a} {e}  `{Ord e} (H : EqLaws e) (f : e -> a -> b) (m : Map e a) lb ub,
   Bounded m lb ub ->
-  (forall k k2 v v2, k == k2 = true -> v = v2 -> f k v = f k2 v2) ->
+  Proper ((fun i j : e => _GHC.Base.==_ i j = true) ==> eq) f ->
   (forall i v, sem (mapWithKey f m) i = Some v -> exists value, sem m i = Some value /\ v = f i value).
 Proof.
   intros. generalize dependent i. generalize dependent v. induction H2; intros.
@@ -72,197 +67,714 @@ Proof.
     destruct Heqo. exists x0. destruct H8. rewrite H8. simpl. split. reflexivity. inversion H7; subst.
     reflexivity. simpl in H7.  assert (sem s1 i = None). { erewrite map_none_spec. apply Heqo. apply H2_. }
     rewrite H8. destruct (i == x) eqn : ?. simpl in H7. simpl. exists v. split. reflexivity. inversion H7. 
-    apply H3. apply Eq_Symmetric. apply Heqb0. reflexivity. simpl. inversion H7. apply IHBounded2.
-    assumption.
+    apply equal_f. apply H3. order e. simpl. simpl in H7. apply IHBounded2. apply H7.
 Qed.
 
 (*If (k,v) is in the original map, then (k, f k v) is in the new map*)
 Lemma map_spec_coq:
-  forall {b} {a} {e} `{Ord e} (H: EqLaws e) (f : e -> a -> b) (m : Map e a) lb ub,
+  forall {b} {a} {e} `{OrdLaws e}(f : e -> a -> b) (m : Map e a) lb ub,
   Bounded m lb ub ->
-  (forall k k2 v v2, k == k2 = true -> v = v2 -> f k v = f k2 v2) ->
+  Proper ((fun i j : e => _GHC.Base.==_ i j = true) ==> eq) f ->
   (forall i v, sem m i = Some v -> sem (mapWithKey f m) i = Some (f i v)).
 Proof.
-  intros.  generalize dependent i. generalize dependent v. induction H2; intros.
-  - inversion H4.
-  - simpl. simpl in H7. destruct (sem s1 i) eqn : ?.
-    * apply IHBounded1 in Heqo. rewrite Heqo. simpl. inversion H7; subst; reflexivity.
-    * assert (sem (mapWithKey f s1) i = None). { erewrite <- map_none_spec. assumption. apply H2_. }
-      simpl in H7. rewrite H8. simpl. destruct (i == x) eqn : ?.
-      + simpl. simpl in H7. inversion H7; subst. erewrite H3. reflexivity. apply Eq_Symmetric.
-        apply Heqb0. reflexivity.
-      + simpl. apply IHBounded2. simpl in H7. assumption.
-Qed.
+  intros. applyDesc e (@mapWithKey_Desc e a). specialize (Hsem i). rewrite H2 in Hsem. assumption.
+Qed. 
 
 (*If f is injective, then (k,v) is in the original map iff (k, f k v) is in the new map*)
 Lemma map_spec_coq_injective:
-  forall {b} {a} {e} `{Ord e} (H: EqLaws e) (f : e -> a -> b) (m : Map e a) lb ub,
+  forall {b} {a} {e} `{OrdLaws e}(f : e -> a -> b) (m : Map e a) lb ub,
   Bounded m lb ub ->
-  (forall k k2 v v2, k == k2 = true -> v = v2 -> f k v = f k2 v2) ->
+  Proper ((fun i j : e => _GHC.Base.==_ i j = true) ==> eq) f ->
   (forall k k2 v v2, f k v = f k2 v2 -> k == k2 = true /\ v = v2) ->
   (forall i v, sem m i = Some v <-> sem (mapWithKey f m) i = Some (f i v)).
 Proof.
-  intros. split.
-  - intros. eapply map_spec_coq; eassumption.
-  - generalize dependent i. generalize dependent v. induction H2; intros.
-    + inversion H2.
-    + simpl in H8. simpl. destruct (sem (mapWithKey f s1) i) eqn : ?.
-      * assert (A:= Heqo). eapply map_spec_reverse in Heqo. destruct Heqo.
-        destruct H9. subst. inversion H8. rewrite H9. simpl.
-        apply H4 in H10. destruct H10. subst. reflexivity. assumption. apply H2_.
-        apply H3.
-      * rewrite <- map_none_spec in Heqo. rewrite Heqo. simpl. simpl in H8. destruct (i == x) eqn : ?.
-        -- simpl. simpl in H8. inversion H8. apply H4 in H10. destruct H10; subst; reflexivity.
-        -- simpl in H8. simpl. apply IHBounded2. assert (A:= H8). eapply map_spec_reverse in H8.
-           assumption. assumption. apply H2_0. assumption.
-        -- apply H2_.
+  intros. applyDesc e (@mapWithKey_Desc e a). specialize (Hsem i). rewrite Hsem.
+  destruct (sem m i); split; intros; inversion H3; try (assumption); try (reflexivity).
+  apply H2 in H5. destruct H5; subst; reflexivity.
 Qed.
 
-(*Specification using Haskell Equality. This requires several lemmas to replace the use
-of [subst] and [rewrite].*)
-
-(*Haskell equality version of [oro_Some_l]*)
-Lemma sem_haskell_eq_some : forall {a} {b} `{EqLaws a} `{EqLaws b} (a1: a) (m : Map a b) b1 o,
-  sem m a1 == Some b1 = true ->
-  (sem m a1 ||| o) == Some b1 = true.
-Proof.
-  intros. destruct (sem m a1) eqn : ?.
-  - simpl. assumption.
-  - inversion H3.
-Qed.
-
-(*Haskell equality version of [oro_None_l]*)
-Lemma sem_haskell_eq_none: forall {a} {b} `{EqLaws a} `{EqLaws b} (a1: a) (m : Map a b) o,
-  sem m a1 == None = true ->
-  (sem m a1 ||| o) == o = true.
-Proof.
-  intros. destruct (sem m a1) eqn : ?.
-  - inversion H3.
-  - simpl. apply Eq_Reflexive.
-Qed.
-
-(*Haskell equality version of [map_none_spec] *)
-Lemma map_none_spec_haskell:
-  forall {b} {a} {e} `{Ord e} (H : EqLaws e) `{EqLaws a} `{EqLaws b} (f: e -> a -> b) (m: Map e a) lb ub,
+(** Verification of [map] *)
+Lemma map_Desc: forall {e} {a} {b} `{OrdLaws e} (m: Map e a) (f: a -> b) lb ub,
   Bounded m lb ub ->
-  (forall i, sem m i == None = true <-> sem (mapWithKey f m) i == None = true).
+  Desc (map f m) lb ub (size m) (fun i => match (sem m i) with
+                                                 | Some x => Some (f x)
+                                                 | None => None end).
 Proof.
-  intros. generalize dependent i. induction H6; intros; split; intros.
-  - simpl. apply Eq_Reflexive. 
-  - simpl. apply Eq_Reflexive. 
-  - simpl. simpl in H10. destruct (sem s1 i) eqn : ?. simpl in H10. inversion H10. simpl in H10.
-    destruct (i == x) eqn : ?. simpl in H10. inversion H10. simpl in H10. destruct (sem s2 i) eqn : ?.
-    inversion H10. apply eq_coq_implies_haskell in Heqo. apply eq_coq_implies_haskell in Heqo0.
-    apply IHBounded1 in Heqo. apply IHBounded2 in Heqo0. rewrite  oro_assoc. simpl.
-    apply (sem_haskell_eq_none _  _ (sem (mapWithKey f s2) i)) in Heqo.
-    eapply Eq_Transitive. apply Heqo. apply Heqo0.
-  - simpl. simpl in H10. destruct (sem (mapWithKey f s1) i) eqn : ?. inversion H10.
-    destruct (i == x) eqn : ?. inversion H10. destruct (sem (mapWithKey f s2) i) eqn : ?.
-    inversion H10. apply eq_coq_implies_haskell in Heqo. apply eq_coq_implies_haskell in Heqo0.
-    simpl. rewrite oro_assoc. simpl. apply IHBounded1 in Heqo. apply IHBounded2 in Heqo0.
-    apply (sem_haskell_eq_none  _ _  (sem s2 i)) in Heqo. eapply Eq_Transitive.
-    apply Heqo. apply Heqo0.
-Qed.
-
-(*Haskell equality version of [map_spec_reverse]*)
-Lemma map_spec_haskell_reverse : 
-  forall {b} {a} {t}  `{Ord t} (H : EqLaws t) `{EqLaws b} `{EqLaws a}
-   (f : t -> a -> b) (m : Map t a) lb ub,
-  Bounded m lb ub ->
-  (forall x1 x2 y1 y2, x1 == x2 = true -> y1 == y2 = true -> f x1 y1 == f x2 y2 = true) ->
-  (forall i v, sem (mapWithKey f m) i == Some v = true -> 
-    exists value, sem m i == Some value = true /\ v == f i value = true).
-Proof.
-  intros.
-  generalize dependent i. generalize dependent v. induction H6; intros.
-  - inversion H8.
-  - simpl in H11. simpl. destruct (sem (mapWithKey f s1) i) eqn : ?.
-    + assert ( _GHC.Base.==_ (sem (mapWithKey f s1) i) (Some b0) = true). { rewrite Heqo.
-      apply Eq_Reflexive. } apply IHBounded1 in H12. destruct H12. exists x0.
-      destruct H12. split. rewrite oro_assoc. apply sem_haskell_eq_some. 
-      apply H12. simpl in H11. rewrite simpl_option_some_eq in H11. eapply Eq_Transitive.
-      apply Eq_Symmetric. apply H11. apply H13.
-    + simpl in H11. apply eq_coq_implies_haskell in Heqo. rewrite <- map_none_spec_haskell in Heqo.
-      destruct (sem s1 i). inversion Heqo. simpl. destruct (i == x) eqn : ?. simpl in H11.
-      simpl. exists v. split. apply Eq_Reflexive. rewrite simpl_option_some_eq in H11. 
-      assert ((f x v) == (f i v) = true). { apply H7. apply Eq_Symmetric. apply Heqb0. 
-      apply Eq_Reflexive. } eapply Eq_Transitive. apply Eq_Symmetric. apply H11. apply H12.
-      simpl. simpl in H11. apply IHBounded2 in H11. apply H11. apply H1. apply H5. apply H3.
-      apply H6_.
+  intros. induction H0.
+  - simpl. solve_Desc e.
+  - simpl. applyDesc e IHBounded1. applyDesc e IHBounded2. solve_Desc e.
 Qed. 
 
-(*A substitute for [rewrite]: If we know a1 == a3, and we have a1 == a2 in the goal, 
-we can prove a2 == a3 instead*)
-Lemma rewrite_eq_haskell : forall {a} `{EqLaws a} a1 a2 a3,
-  a1 == a2 = true -> (a1 == a3 = true <-> a2 == a3 = true).
-Proof.
-  intros; split; intros.
-  - eapply Eq_Transitive. apply Eq_Symmetric. apply H1. apply H2.
-  - eapply Eq_Transitive. apply H1. apply H2.
-Qed.
-
-(*Specification for mapWithKey using Haskell equality*)
-Lemma map_spec_haskell:
-  forall {b} {a} {e} `{Ord e} (H: EqLaws e) `{EqLaws b} `{EqLaws a} (f : e -> a -> b) (m : Map e a) lb ub,
-  Bounded m lb ub ->
-  (forall x1 x2 y1 y2, x1 == x2 = true -> y1 == y2 = true -> f x1 y1 == f x2 y2 = true) ->
-  (forall i v, sem m i == Some v = true -> sem (mapWithKey f m) i == Some (f i v) = true).
-Proof.
-  intros.  generalize dependent i. generalize dependent v. induction H6; intros.
-  - inversion H8.
-  - simpl. simpl in H11. destruct (sem s1 i) eqn : ?.
-    * apply eq_coq_implies_haskell in Heqo. apply IHBounded1 in Heqo. rewrite oro_assoc.
-      eapply sem_haskell_eq_some. simpl in H11. rewrite simpl_option_some_eq in H11.
-      assert (f i a0 == f i v0 = true). { apply H7. apply Eq_Reflexive. apply H11. }
-      eapply Eq_Transitive. apply Heqo. rewrite simpl_option_some_eq. apply H12.
-    * apply eq_coq_implies_haskell in Heqo. erewrite map_none_spec_haskell in Heqo.
-      rewrite oro_assoc. eapply (sem_haskell_eq_none i (mapWithKey f s1)
-      (SomeIf (_GHC.Base.==_ i x) (f x v) ||| sem (mapWithKey f s2) i)) in Heqo.
-      (*rewrite to make the goal simpler*)
-      assert (_GHC.Base.==_ (sem (mapWithKey f s1) i ||| 
-      (SomeIf (_GHC.Base.==_ i x) (f x v) ||| sem (mapWithKey f s2) i))
-      (Some (f i v0)) = true <-> ((SomeIf (_GHC.Base.==_ i x) (f x v) ||| 
-      sem (mapWithKey f s2) i) == Some (f i v0) = true)).
-      apply rewrite_eq_haskell. apply Heqo. rewrite H12. clear H12.
-      destruct (i == x) eqn : ?. simpl. simpl in H11. rewrite simpl_option_some_eq.
-      apply H7. apply Eq_Symmetric. apply Heqb0. rewrite simpl_option_some_eq in H11. apply H11.
-      simpl. apply IHBounded2. simpl in H11. apply H11. assumption. assumption. assumption.
-      apply H6_.
-Qed.
-
-(*Once again. if f is injective, we get a stronger claim*)
-Lemma map_spec_haskell_injective:
-  forall {b} {a} {e} `{Ord e} (H: EqLaws e) `{EqLaws b} `{EqLaws a} (f : e -> a -> b) (m : Map e a) lb ub,
-  Bounded m lb ub ->
-  (forall x1 x2 y1 y2, x1 == x2 = true -> y1 == y2 = true -> f x1 y1 == f x2 y2 = true) ->
-  (forall k k2 v v2, f k v == f k2 v2 = true -> k == k2 = true /\ v = v2) ->
-  (forall i v, sem m i == Some v = true <-> sem (mapWithKey f m) i == Some (f i v) = true).
-Proof.
-  intros. split.
-  - intros. eapply map_spec_haskell; eassumption.
-  - generalize dependent i. generalize dependent v. induction H6; intros.
-    + inversion H6.
-    + simpl in H12. simpl. destruct (sem (mapWithKey f s1) i) eqn : ?.
-      * assert (A:= Heqo). apply eq_coq_implies_haskell in Heqo. eapply map_spec_haskell_reverse in Heqo.
-        destruct Heqo. destruct H13. simpl in H12. 
-        apply eq_coq_implies_haskell in A. assert ( (sem (mapWithKey f s1) i) == (Some (f i v0)) = true).
-        { eapply Eq_Transitive. apply A. apply H12. } apply IHBounded1 in H15.
-         rewrite oro_assoc. eapply sem_haskell_eq_some. apply H15. assumption. assumption.
-        apply H5. apply H6_. assumption.
-      * apply eq_coq_implies_haskell in Heqo. rewrite <- map_none_spec_haskell in Heqo.
-        destruct (sem s1 i). inversion Heqo. simpl. simpl in H12. destruct (i== x) eqn : ?.
-        -- simpl. simpl in H12. apply H8 in H12. destruct H12; subst; apply Eq_Reflexive.
-        -- simpl. simpl in H12. apply IHBounded2. apply H12.
-        -- assumption.
-        -- apply H5.
-        -- assumption.
-        -- apply H6_.
-Qed.
-
-Lemma map_no_key_spec :  forall {e} {a} {b} `{Ord e} (f : a -> b) (m : Map e a),
+Lemma map_mapWithKey_equiv:  forall {e} {a} {b} `{Ord e} (f : a -> b) (m : Map e a),
   Internal.map f m = mapWithKey (fun k v => f v) m.
 Proof.
   intros. induction m.
   - simpl. rewrite IHm1. rewrite IHm2. reflexivity.
   - simpl. reflexivity.
 Qed.
+
+(** Vertification of [mapAccumL] *)
+
+(*This turns out to be highly nontrivial to specify and verify. At each step, the new value is calculated
+based on a function that uses the old key and the accumulated value through all of the previous keys. 
+We can specify the value by stating that it is euivalent to folding the function over the map,
+but the resulting map is much harder to specify, and the proof is quite complex*)
+
+
+Lemma mapAccumL_fst: forall {e} {a} {b : Type} {c : Type} `{OrdLaws e} (m: Map e a) (x : b) 
+  (f: b -> e -> a -> (b * c)) lb ub,
+   Bounded m lb ub ->
+  fst(mapAccumL f x m) = foldlWithKey (fun (t: b) k v => fst (f t k v)) x m.
+Proof.
+  intros. revert x. induction H0; intros.
+  - simpl. reflexivity.
+  - simpl. rewrite (surjective_pairing (mapAccumL f x0 s1 )).
+    rewrite (surjective_pairing (mapAccumL f x0 s1)). simpl.
+    rewrite IHBounded1. 
+    rewrite (surjective_pairing (f (foldlWithKey (fun (t : b) (k : e) (v0 : a) => fst (f t k v0)) x0 s1) x v )).
+    simpl. 
+    rewrite (surjective_pairing (mapAccumL f (fst (f (foldlWithKey (fun (t : b) (k : e) (v0 : a) => 
+    fst (f t k v0)) x0 s1) x v)) s2 )). simpl. rewrite IHBounded2. reflexivity.
+Qed.
+
+(*In order to specify the resulting map, we need a way to describe the accumulated value. We do this
+by claiming that the accumulated value is equivalent to folding the function over every element in the
+map less than the current key. To specify this, we define map_lt, which consists of all elements
+in the map less than the current key. We then prove a Desc about it*)
+Definition map_lt {e} `{Ord e} {a} (m: Map e a) k :=
+  fst(partitionWithKey (fun x _ => x < k) m).
+
+Lemma map_lt_Desc: forall {e a} `{OrdLaws e}  (m: Map e a) k lb ub,
+  Bounded m lb ub ->
+  Desc' (map_lt m k) lb ub (fun i => if i < k then sem m i else None).
+Proof.
+  intros. unfold map_lt. induction H0.
+  - simpl. solve_Desc e. f_solver e.
+  - eapply (@partitionWithKey_spec e a). assumption. constructor. apply H0_. apply H0_0.
+    assumption. assumption. assumption. assumption. unfold respectful. unfold Proper.
+    intros. assert ( _GHC.Base.<_ x0 k =  _GHC.Base.<_ y k ) by (order e). 
+    rewrite H5. reflexivity. intros. simpl. applyDesc e H4. solve_Desc e. f_solver e.
+    destruct (sem s1 i); simpl in Hsem. inversion Hsem. destruct (i == x); simpl in Hsem.
+    inversion Hsem. destruct (sem s2 i); inversion Hsem.
+Qed.  
+
+(*The key issue in the resulting proof is that we have something like
+[forall i, sem s4 i = sem s1 i ||| SomeIf (i == x) v ||| sem s3 i]
+and we want to prove that folding over s1, then x, then s3 is the same as folding over s4.
+This turns out to be very complicated, and is slightly easier to reason about if we use lists
+instead. The next several lemmas allow us to do this.*) 
+
+(*TODO: Move this to toListProofs. The one in toListProofs is not sufficiently general*)
+Lemma foldlWithKey_spec' :
+   forall (e a b : Type) (f : b -> e -> a -> b) (n : b) (m : Map e a),
+   foldlWithKey f n m = fold_left (fun t (x: e * a) => let (a0, b) := x in f t a0 b) (toList m) n.
+Proof.
+  intros. generalize dependent n. induction m; intros.
+  - simpl. rewrite toList_Bin. rewrite IHm1. rewrite IHm2.
+    rewrite fold_left_app. simpl. reflexivity.
+  - reflexivity.
+Qed.
+
+
+(*I don't think the {EqLaws a} assumption is strictly necessary, but it is difficult to remove, 
+since the proofs rely on theorems about toList and equality that would have to be re-proved
+without reference to EqLaws*)
+Lemma fold_left_proper: 
+  forall {e} {a} {b} `{OrdLaws e} `{EqLaws a} (f: b -> e * a -> b) x (l1 l2: list (e * a)),
+  eqlist l1 l2 = true ->
+  (forall p1 p2 y, p1 == p2 = true -> f y p1 = f y p2) ->
+  (fold_left f l1 x) = (fold_left f l2 x).
+Proof.
+  intros. revert x. generalize dependent l2. induction l1; intros; destruct l2.
+  - reflexivity.
+  - inversion H2.
+  - inversion H2.
+  - simpl. simpl in H2. 
+    assert (f x a0 = f x p). apply H3. order e. rewrite H4. apply IHl1. 
+    rewrite andb_true_iff in H2. destruct H2. assumption.
+Qed.
+
+(*The result we really need about fold: If we have maps that are equivalent sem-wise,
+then folding over them gives the same result (assuming the function is Proper)*)
+Lemma foldlWithKey_equiv_maps:
+  forall {e} {a} {b} `{OrdLaws e} `{EqLaws a} (f: b -> e -> a -> b) x (m1: Map e a) m2, 
+  WF m1 ->
+  WF m2 ->
+  (forall e1 e2 a1 a2 y, a1 == a2 = true -> e1 == e2 = true -> f y e1 a1 = f y e2 a2) ->
+  (forall i, sem m1 i = sem m2 i) ->
+  (foldlWithKey f x m1) = (foldlWithKey f x m2).
+Proof.
+  intros. rewrite foldlWithKey_spec'. rewrite foldlWithKey_spec'.
+  assert (eqlist (toList m1) (toList m2) = true). { 
+  assert ((toList m1) == (toList m2) = true).
+  assert (m1 == m2 = true) by (eapply strong_eq1; eassumption).
+  unfold "==" in H6. unfold Eq___Map in H6. unfold op_zeze____ in H6.
+  unfold Internal.Eq___Map_op_zeze__ in H6. unfold toList. rewrite andb_true_iff in H6.
+  destruct H6. assumption. unfold "==" in H6. unfold Eq_list in H6. unfold op_zeze____ in H6.
+  apply H6. } apply fold_left_proper. apply H6. intros.
+  destruct p1. destruct p2. unfold "==" in H7. unfold Eq_pair___  in H7. 
+  unfold op_zeze____  in H7. unfold eq_pair in H7. rewrite andb_true_iff in H7. apply H4.
+  order a. order e.
+Qed. 
+
+
+(*TODO: PUT THIS IN BOUNDS*)
+(*Some lemmas and ltac to prove that any m such that Bounded m lb ub is well formed*)
+
+Lemma expand_bounds_l : forall {e} {a} `{OrdLaws e} (m: Map e a) lb x,
+  Bounded m lb x ->
+  Bounded m None x.
+Proof.
+  intros. induction H0.
+  - constructor.
+  - constructor; try (reflexivity); try (assumption).
+Qed.
+
+Lemma expand_bounds_r : forall {e a} `{OrdLaws e} (m: Map e a) ub x,
+  Bounded m x ub ->
+  Bounded m x None.
+Proof.
+  intros. induction H0.
+  - constructor.
+  - constructor; try (reflexivity); try (assumption).
+Qed.
+
+Ltac wf_bounds:= eapply expand_bounds_l; eapply expand_bounds_r; eassumption.
+
+Require Import Coq.Sorting.Sorted.
+
+(*A few lemmas about the Boundedness of lists*)
+(*TODO:Move to toListProofs*)
+Lemma toList_Bounds_UB: forall {e} {a} `{OrdLaws e} (m: Map e a) lb ub, 
+  Bounded m lb ub -> 
+  forall k v, In (k,v) (toList m) ->
+  isUB ub k = true.
+Proof.
+  intros. induction H0. inversion H1. rewrite toList_Bin in H1.
+  apply in_app_or in H1. destruct H1. apply IHBounded1 in H1. solve_Bounds e. simpl in H1.
+  destruct H1. solve_Bounds e. apply IHBounded2. assumption.
+Qed. 
+
+Lemma toList_Bounds_LB: forall {e} {a} `{OrdLaws e} (m: Map e a) lb ub, 
+  Bounded m lb ub -> 
+  forall k v, In (k,v) (toList m) ->
+  isLB lb k = true.
+Proof.
+  intros. induction H0. inversion H1. rewrite toList_Bin in H1.
+  apply in_app_or in H1. destruct H1. apply IHBounded1. assumption.  simpl in H1.
+  destruct H1. solve_Bounds e. apply IHBounded2 in H1. solve_Bounds e.
+Qed.
+
+Lemma eq_list_equiv: forall {a} `{EqLaws a} (l1 l2 : list a),
+  l1 == l2 = eqlist l1 l2.
+Proof.
+  intros. unfold "==". unfold Eq_list. unfold op_zeze____. reflexivity.
+Qed.
+
+Set Bullet Behavior "Strict Subproofs".
+(*TODO: Also somewhere else*)
+(*If a list is sorted, sem_for_lists gives Some x on i iff (i,x) is in the list (the converse is
+not true unless the list has unique elements)*)
+Lemma sem_to_lists_elem: forall {e} {a} `{OrdLaws e} `{EqLaws a} (l: list (e * a)) i x,
+  StronglySorted ToListProofs.lt l ->
+ (sem_for_lists l i == Some x) = true <-> List.elem (i, x) l = true.
+Proof. 
+  intros. revert H2. revert i x. induction l; intros.
+    - simpl. split; intros contra; inversion contra. 
+    - simpl. destruct a0. split; intros.
+      + destruct (i == e0) eqn : ?. 
+      rewrite orb_true_iff. left. unfold "==". unfold Eq_pair___. unfold op_zeze____.
+      unfold eq_pair. rewrite andb_true_iff. split. assumption. apply Eq_Symmetric.
+      rewrite simpl_option_some_eq in H3. apply H3.
+      rewrite orb_true_iff. right. erewrite <- IHl. assumption. inversion H2; assumption.
+      + rewrite orb_true_iff in H3. destruct H3.
+        * unfold "==" in H3. unfold Eq_pair___ in H3. unfold op_zeze____ in H3.
+          unfold eq_pair in H3. rewrite andb_true_iff in H3. destruct H3. rewrite H3.
+          rewrite simpl_option_some_eq. order a.
+        * inversion H2; subst. rewrite Forall_lt in H7. specialize (H7 i x). assert (A:=H3).
+          apply H7 in H3. unfold ToListProofs.lt in H3. assert (i == e0 = false) by (order e).
+          rewrite H4. rewrite  IHl. apply A. apply H6.
+Qed. 
+
+Lemma fromDistinctAscList_toList: forall {e} {a} `{OrdLaws e} `{EqLaws a} (l: list (e * a)), 
+  StronglySorted ToListProofs.lt l -> 
+  toList(fromDistinctAscList l) == l = true.
+Proof.
+  intros. apply strongly_sorted_unique.
+  - eapply to_List_sorted. eapply fromDistinctAscList_Desc. apply H2. intros. apply H3.
+  - apply H2.
+  - intros. eapply fromDistinctAscList_Desc. apply H2. intros.
+    split; intros.
+    + rewrite <- toList_sem' in H6. destruct (sem s x) eqn : ?.
+      * apply sem_to_lists_elem. apply H2. rewrite H5 in Heqo. rewrite Heqo. assumption.
+      * inversion H6.
+      * apply H3.
+    + rewrite <- sem_to_lists_elem in H6. destruct (sem_for_lists l x) eqn : ?. specialize (H5 x).
+      rewrite <- toList_sem'. rewrite H5. rewrite Heqo. assumption. apply H3. inversion H6. apply H2.
+Qed.
+
+Ltac unfold_pair := unfold "==" ; unfold Eq_pair___ ; unfold op_zeze____ ; unfold eq_pair. 
+
+
+(*Finally, the actual specification, which says that any element is found by computing f on the
+accumulated value (value resulting from folding f over all elements less than f) and the key itself.
+Again, I'm not sure if the {EqLaws a} assumption is strictly needed*)
+Lemma mapAccumL_snd_Desc: forall {e} {a} {b : Type} {c : Type} `{OrdLaws e} `{EqLaws a} (m: Map e a) (x : b) 
+  (f: b -> e -> a -> (b * c)) lb ub,
+  Proper ((fun (i j : e * a) => _GHC.Base.==_ i j = true) ==> eq) (fun x y => let (a,b) := x in f y a b) ->
+  Bounded m lb ub ->
+  Desc (snd (mapAccumL f x m)) lb ub (size m) (
+  fun i => match (sem m i) with
+           | Some y => Some (snd(f (fst (mapAccumL f x (map_lt m i))) i y))
+           | None => None
+            end).
+Proof.
+  intros. revert x. induction H3; intros.
+  - simpl. solve_Desc e.
+  - simpl.  rewrite (surjective_pairing (mapAccumL f x0 s1 )).
+    rewrite (surjective_pairing (f (fst (mapAccumL f x0 s1)) x v)).
+    rewrite (surjective_pairing ( mapAccumL f (fst (f (fst (mapAccumL f x0 s1)) x v)) s2)).
+    simpl. applyDesc e IHBounded1. applyDesc e IHBounded2. solve_Desc e. f_solver e.
+    + repeat(applyDesc e (@map_lt_Desc e a)). repeat (erewrite mapAccumL_fst).
+      * assert (forall i, sem s4 i = sem s3 i). {
+         intros. destruct (_GHC.Base.<_ i0 i) eqn : ?.
+          - specialize (Hsem1 i0). rewrite Heqb0 in Hsem1. simpl in Hsem1.
+            assert (i0 == x = false) by (solve_Bounds e). assert (sem s2 i0 = None). eapply sem_outside_below.
+            eassumption. solve_Bounds e. rewrite H7 in Hsem1. rewrite H5 in Hsem1. simpl in Hsem1. 
+            repeat (rewrite oro_None_r in Hsem1). rewrite Hsem1. rewrite Hsem.
+            rewrite Heqb0. reflexivity.
+          - specialize (Hsem1 i0). specialize (Hsem i0). rewrite Hsem. rewrite Hsem1. rewrite Heqb0. 
+            reflexivity. }
+        assert ((foldlWithKey (fun (t : b) (k : e) (v0 : a) => fst (f t k v0)) x0 s3) =
+           (foldlWithKey (fun (t : b) (k : e) (v0 : a) => fst (f t k v0)) x0 s4)). {
+            eapply foldlWithKey_equiv_maps. wf_bounds. wf_bounds. intros.
+            assert (f y e1 a1 = f y e2 a2). { unfold respectful in H2. unfold Proper in H2.
+            remember (e1, a1). remember (e2, a2). assert (p == p0 = true). unfold_pair.
+            subst. rewrite andb_true_iff. split; assumption. apply H2 in H9. subst.
+            eapply equal_f in H9. apply H9. } rewrite H9. reflexivity.
+            intros. rewrite H5. reflexivity. }
+        rewrite H7. reflexivity.
+      * eassumption.
+      * eassumption.
+    + applyDesc e (@map_lt_Desc e a). repeat (erewrite mapAccumL_fst).
+      * assert (forall i, sem s1 i = sem s3 i). {
+        intros. destruct (_GHC.Base.<_ i0 i) eqn : ?.
+        - specialize (Hsem i0). rewrite Heqb1 in Hsem. simpl in Hsem.
+          assert (i0 == x = false) by (solve_Bounds e). assert (sem s2 i0 = None). eapply sem_outside_below.
+          eassumption. solve_Bounds e. rewrite H8 in Hsem. rewrite H7 in Hsem. simpl in Hsem. 
+          repeat (rewrite oro_None_r in Hsem). rewrite Hsem. reflexivity.
+        - specialize (Hsem i0). rewrite Hsem.  rewrite Heqb1. eapply sem_outside_above. eassumption.
+          solve_Bounds e. }  
+        assert ((foldlWithKey (fun (t : b) (k : e) (v0 : a) => fst (f t k v0)) x0 s1) =
+           (foldlWithKey (fun (t : b) (k : e) (v0 : a) => fst (f t k v0)) x0 s3)). {
+          eapply foldlWithKey_equiv_maps. wf_bounds. wf_bounds. intros.
+          assert (f y e1 a1 = f y e2 a2). { unfold respectful in H2. unfold Proper in H2.
+          remember (e1, a1). remember (e2, a2). assert (p == p0 = true). unfold_pair.
+          subst. rewrite andb_true_iff. split; assumption. apply H2 in H10. subst.
+          eapply equal_f in H10. apply H10. } rewrite H10. reflexivity. 
+          intros. rewrite H7. reflexivity. }
+      rewrite H8. assert (forall z, f z x v = f z i v). { intros. unfold respectful in H2.
+        unfold Proper in H2. remember (x, v). remember (i,v).
+        assert (p == p0 = true). unfold_pair. subst. rewrite andb_true_iff. split. order e. order a.
+        apply H2 in H9. subst. eapply equal_f in H9. apply H9. }
+      rewrite H9. reflexivity.
+     * eassumption.
+     * eassumption.
+    + (*This case is the complicated one that involves all sorts of results about fold, toList, and 
+        fromDistinctAscList*)
+    remember ((1 + size s1 + size s2)%Z) as sz. repeat (applyDesc e (@map_lt_Desc e a)).
+    repeat (erewrite mapAccumL_fst). repeat (rewrite foldlWithKey_spec').
+    assert
+        ((fold_left (fun (t : b) (x1 : e * a) => let (a1, b0) := x1 in fst (f t a1 b0)) 
+           (toList s3)
+           (fst
+              (f (fold_left (fun (t : b) (x1 : e * a) => let (a1, b0) := x1 in fst (f t a1 b0)) (toList s1) x0) x
+                 v))) = fold_left (fun (t : b) (x1 : e * a) => let (a1, b0) := x1 in fst (f t a1 b0)) 
+                  ((toList s1) ++ ((x, v) :: nil) ++ (toList s3)) x0). { simpl.
+    rewrite fold_left_app. simpl. reflexivity. }
+    rewrite H5. clear H5. 
+    assert ((fold_left (fun (t : b) (x1 : e * a) => let (a1, b0) := x1 in fst (f t a1 b0))
+           (toList s1 ++ ((x, v) :: nil) ++ toList s3) x0) = 
+    (fold_left (fun (t : b) (x1 : e * a) => let (a1, b0) := x1 in fst (f t a1 b0)) (toList s4) x0) ). {
+      assert (StronglySorted ToListProofs.lt (toList s1 ++ ((x, v) :: nil) ++ toList s3)). {
+        eapply sorted_append.
+        + eapply to_List_sorted. eassumption.
+        + simpl. apply SSorted_cons.
+          * eapply to_List_sorted. eassumption.
+          * rewrite Forall_lt. intros. unfold ToListProofs.lt. rewrite <- toList_sem' in H5.
+            destruct (sem s3 x1) eqn : ?.
+            - solve_Bounds e.
+            - inversion H5.
+            - eassumption.
+       + intros. assert (isUB (Some x) y = true). eapply toList_Bounds_UB. apply H3_. apply H5. solve_Bounds e.
+       + intros. simpl in H5. destruct H5.
+          * inversion H5; subst. order e.
+          * assert (isLB (Some x) y = true). eapply toList_Bounds_LB. apply HB1. apply H5. solve_Bounds e. }
+      eapply fold_left_proper.
+      - simpl. remember (fromDistinctAscList ((toList s1 ++ ((x, v) :: nil) ++ toList s3))) as m.
+        assert (toList m ==  (toList s1 ++ ((x, v) :: nil) ++ toList s3) = true). { rewrite Heqm.
+        eapply fromDistinctAscList_toList. apply H5. }
+        rewrite <- eq_list_equiv. eapply Eq_Transitive. apply Eq_Symmetric. apply H7.
+        unfold is_true. rewrite <-eq_toList. eapply strong_eq1.
+        + subst. eapply fromDistinctAscList_Desc. apply H5. intros. apply H8.
+        + wf_bounds.
+        + intros. rewrite Hsem0. rewrite Heqm. eapply fromDistinctAscList_Desc. apply H5. intros.
+          rewrite H10. simpl. rewrite sem_list_app.
+          destruct (i0 < i) eqn : ?.
+          * erewrite <- toList_sem''. simpl. unfold SomeIf.  erewrite <- toList_sem''.
+            rewrite Hsem. rewrite Heqb1. 
+            destruct (sem s1 i0).
+            -- reflexivity.
+            -- destruct (i0 == x); reflexivity.
+            -- eassumption.
+            -- eassumption.
+          * erewrite <- toList_sem''. destruct (sem s1 i0) eqn : ?.
+            -- solve_Bounds e.
+            -- simpl. destruct (i0 == x) eqn : ?.
+               ++ solve_Bounds e.
+               ++ erewrite <- toList_sem''. rewrite Hsem. rewrite Heqb1. reflexivity.
+                  eassumption.
+            -- eassumption.
+        + rewrite Heqm. apply fromDistinctAscList_Desc. apply H5. intros. apply H8.
+        + wf_bounds.
+      - intros. apply H2 in H7. destruct p1. destruct p2.
+        eapply equal_f in H7. rewrite H7. reflexivity. }
+    rewrite H5. reflexivity. apply HB2. apply H3_. apply HB1.
+Qed. 
+
+(** Verification of [mapAccumWithKey] *)
+
+(*This is much simpler*)
+Lemma mapAccumWithKey_mapAccumL: forall {e} {a} {b : Type} {c : Type} `{OrdLaws e} (m: Map e a) (x : b) 
+  (f: b -> e -> a -> (b * c)),
+  mapAccumWithKey f x m = mapAccumL f x m.
+Proof.
+  intros. unfold mapAccumWithKey. reflexivity.
+Qed.
+
+Lemma mapAccumWithKey_fst: forall {e} {a} {b : Type} {c : Type} `{OrdLaws e} (m: Map e a) (x : b) 
+  (f: b -> e -> a -> (b * c)) lb ub,
+   Bounded m lb ub ->
+  fst(mapAccumWithKey f x m) = foldlWithKey (fun (t: b) k v => fst (f t k v)) x m.
+Proof.
+  intros. rewrite mapAccumWithKey_mapAccumL. eapply mapAccumL_fst. apply H0.
+Qed.
+
+Lemma mapAccumWithKey_snd_Desc: forall {e} {a} {b : Type} {c : Type} `{OrdLaws e} `{EqLaws a} (m: Map e a) (x : b) 
+  (f: b -> e -> a -> (b * c)) lb ub,
+  Proper ((fun (i j : e * a) => _GHC.Base.==_ i j = true) ==> eq) (fun x y => let (a,b) := x in f y a b) ->
+  Bounded m lb ub ->
+  Desc (snd (mapAccumWithKey f x m)) lb ub (size m) (
+  fun i => match (sem m i) with
+           | Some y => Some (snd(f (fst (mapAccumWithKey f x (map_lt m i))) i y))
+           | None => None
+            end).
+Proof.
+  intros. repeat(setoid_rewrite mapAccumWithKey_mapAccumL). eapply (@mapAccumL_snd_Desc e a); assumption.
+Qed.
+
+(** Verification of [mapAccum] *)
+Lemma mapAccum_mapAccumWithKey: forall {e} {a} {b : Type} {c : Type} `{OrdLaws e} (m: Map e a) (x : b) 
+  (f: b ->  a -> (b * c)),
+  mapAccum f x m = mapAccumWithKey (fun a b c => f a c) x m.
+Proof.
+  intros. unfold mapAccum. reflexivity.
+Qed.
+
+Lemma mapAccum_fst: forall {e} {a} {b : Type} {c : Type} `{OrdLaws e} (m: Map e a) (x : b) 
+  (f: b -> a -> (b * c)) lb ub,
+   Bounded m lb ub ->
+  fst(mapAccum f x m) = foldlWithKey (fun (t: b) k v => fst (f t v)) x m.
+Proof.
+  intros. rewrite mapAccum_mapAccumWithKey. eapply mapAccumWithKey_fst. apply H0.
+Qed.
+
+Lemma mapAccum_snd_Desc: forall {e} {a} {b : Type} {c : Type} `{OrdLaws e} `{EqLaws a} (m: Map e a) (x : b) 
+  (f: b -> a -> (b * c)) lb ub,
+  Proper ((fun (i j : a) => _GHC.Base.==_ i j = true) ==> eq) (fun x y =>  f y x) ->
+  Bounded m lb ub ->
+  Desc (snd (mapAccum f x m)) lb ub (size m) (
+  fun i => match (sem m i) with
+           | Some y => Some (snd(f (fst (mapAccum f x (map_lt m i))) y))
+           | None => None
+            end).
+Proof.
+  intros. repeat(setoid_rewrite mapAccum_mapAccumWithKey). eapply (@mapAccumWithKey_snd_Desc e a).
+  all: try (assumption). unfold respectful. unfold Proper. unfold_pair. intros. destruct x0. destruct y.
+  apply H2. order a. 
+Qed.
+
+(** Verification of [mapAccumRWithKey] *)
+(*This is the reverse of [mapAccumL] (fold right instead of left)*)
+Lemma mapAccumRWithKey_fst: forall {e} {a} {b : Type} {c : Type} `{OrdLaws e} (m: Map e a) (x : b) 
+  (f: b -> e -> a -> (b * c)) lb ub,
+   Bounded m lb ub ->
+  fst(mapAccumRWithKey f x m) = foldrWithKey (fun k v t => fst (f t k v)) x m.
+Proof.
+  intros. revert x. induction H0; intros.
+  - simpl. reflexivity.
+  - simpl. rewrite (surjective_pairing (mapAccumRWithKey f x0 s2 )).
+    rewrite (surjective_pairing (mapAccumRWithKey f x0 s2)). simpl.
+    rewrite IHBounded2. 
+    rewrite (surjective_pairing (f (foldrWithKey (fun (k : e) (v0 : a) (t: b) => fst (f t k v0)) x0 s2) x v )).
+    simpl. 
+    rewrite (surjective_pairing (mapAccumRWithKey f (fst (f (foldrWithKey (fun (k : e) (v0 : a)  (t : b) => 
+    fst (f t k v0)) x0 s2) x v)) s1 )). simpl. rewrite IHBounded1. reflexivity.
+Qed.
+
+Definition map_gt {e} `{Ord e} {a} (m: Map e a) k :=
+  fst(partitionWithKey (fun x _ => x > k) m).
+
+Lemma map_gt_Desc: forall {e a} `{OrdLaws e}  (m: Map e a) k lb ub,
+  Bounded m lb ub ->
+  Desc' (map_gt m k) lb ub (fun i => if i > k then sem m i else None).
+Proof.
+  intros. unfold map_gt. induction H0.
+  - simpl. solve_Desc e. f_solver e.
+  - eapply (@partitionWithKey_spec e a). assumption. constructor. apply H0_. apply H0_0.
+    assumption. assumption. assumption. assumption. unfold respectful. unfold Proper.
+    intros. assert ( _GHC.Base.>_ x0 k =  _GHC.Base.>_ y k ) by (order e). 
+    rewrite H5. reflexivity. intros. simpl. applyDesc e H4. solve_Desc e. f_solver e.
+    destruct (sem s1 i); simpl in Hsem. inversion Hsem. destruct (i == x); simpl in Hsem.
+    inversion Hsem. destruct (sem s2 i); inversion Hsem.
+Qed.  
+
+(*TODO: Move this to toListProofs. The one in toListProofs is not sufficiently general*)
+Lemma foldrWithKey_spec' :
+   forall (e a b : Type) (f :  e -> a -> b -> b) (n : b) (m : Map e a),
+   foldrWithKey f n m = fold_right (fun (x: e * a) t => let (a0, b) := x in f a0 b t) n (toList m).
+Proof.
+  intros. generalize dependent n. induction m; intros.
+  - simpl. rewrite toList_Bin. rewrite IHm1. rewrite IHm2.
+    rewrite fold_right_app. simpl. reflexivity.
+  - reflexivity.
+Qed.
+
+
+Lemma fold_right_proper: 
+  forall {e} {a} {b} `{OrdLaws e} `{EqLaws a} (f: e * a -> b -> b) x (l1 l2: list (e * a)),
+  eqlist l1 l2 = true ->
+  (forall p1 p2 y, p1 == p2 = true -> f p1 y = f p2 y) ->
+  (fold_right f x l1) = (fold_right f x l2).
+Proof.
+  intros. revert x. generalize dependent l2. induction l1; intros; destruct l2.
+  - reflexivity.
+  - inversion H2.
+  - inversion H2.
+  - simpl. simpl in H2. specialize (IHl1 l2). rewrite andb_true_iff in H2.
+    destruct H2. rewrite IHl1. apply H3. assumption. assumption. 
+Qed. 
+
+Lemma foldRWithKey_equiv_maps:
+  forall {e} {a} {b} `{OrdLaws e} `{EqLaws a} (f: e -> a -> b -> b) x (m1: Map e a) m2, 
+  WF m1 ->
+  WF m2 ->
+  (forall e1 e2 a1 a2 y, a1 == a2 = true -> e1 == e2 = true -> f e1 a1 y = f e2 a2 y) ->
+  (forall i, sem m1 i = sem m2 i) ->
+  (foldrWithKey f x m1) = (foldrWithKey f x m2).
+Proof.
+  intros. rewrite foldrWithKey_spec'. rewrite foldrWithKey_spec'.
+  assert (eqlist (toList m1) (toList m2) = true). { 
+  assert ((toList m1) == (toList m2) = true).
+  assert (m1 == m2 = true) by (eapply strong_eq1; eassumption).
+  unfold "==" in H6. unfold Eq___Map in H6. unfold op_zeze____ in H6.
+  unfold Internal.Eq___Map_op_zeze__ in H6. unfold toList. rewrite andb_true_iff in H6.
+  destruct H6. assumption. unfold "==" in H6. unfold Eq_list in H6. unfold op_zeze____ in H6.
+  apply H6. } apply fold_right_proper. apply H6. intros.
+  destruct p1. destruct p2. unfold "==" in H7. unfold Eq_pair___  in H7. 
+  unfold op_zeze____  in H7. unfold eq_pair in H7. rewrite andb_true_iff in H7.
+  apply H4. 
+  order a. order e.
+Qed. 
+
+Lemma mapAccumRWithKey_Desc: forall {e} {a} {b : Type} {c : Type} `{OrdLaws e} `{EqLaws a} (m: Map e a) (x : b) 
+  (f: b -> e -> a -> (b * c)) lb ub,
+  Proper ((fun (i j : e * a) => _GHC.Base.==_ i j = true) ==> eq) (fun x y => let (a,b) := x in f y a b) ->
+  Bounded m lb ub ->
+  Desc (snd (mapAccumRWithKey f x m)) lb ub (size m) (
+  fun i => match (sem m i) with
+           | Some y => Some (snd(f (fst (mapAccumRWithKey f x (map_gt m i))) i y))
+           | None => None
+            end).
+Proof.
+  intros. revert x. induction H3; intros.
+  - simpl. solve_Desc e.
+  - simpl.  rewrite (surjective_pairing (mapAccumRWithKey f x0 s2 )).
+    rewrite (surjective_pairing (f (fst (mapAccumRWithKey f x0 s2)) x v)).
+    rewrite (surjective_pairing ( mapAccumRWithKey f (fst (f (fst (mapAccumRWithKey f x0 s2)) x v)) s1)).
+    simpl. applyDesc e IHBounded1. applyDesc e IHBounded2. solve_Desc e. f_solver e.
+    + (*This case is the complicated one that involves all sorts of results about fold, toList, and 
+        fromDistinctAscList*)
+    remember ((1 + size s1 + size s2)%Z) as sz. repeat (applyDesc e (@map_gt_Desc e a)).
+    repeat (erewrite mapAccumRWithKey_fst). repeat (rewrite foldrWithKey_spec').
+    assert(
+        (fold_right (fun (x1 : e * a) (t : b) => let (a1, b0) := x1 in fst (f t a1 b0))
+           (fst
+              (f (fold_right (fun (x1 : e * a) (t : b) => let (a1, b0) := x1 in fst (f t a1 b0)) x0 (toList s2))
+                 x v)) (toList s3)) =
+        fold_right (fun (x1 : e * a) (t : b) => let (a1, b0) := x1 in fst (f t a1 b0)) 
+         x0 ((toList s3) ++ ((x, v) :: nil) ++ (toList s2))). { simpl. rewrite fold_right_app.
+         simpl. reflexivity. }
+    rewrite H5. clear H5. 
+    assert ((fold_right (fun  (x1 : e * a) (t : b) => let (a1, b0) := x1 in fst (f t a1 b0)) x0
+           (toList s3 ++ ((x, v) :: nil) ++ toList s2)) = 
+    (fold_right (fun(x1 : e * a)  (t : b)  => let (a1, b0) := x1 in fst (f t a1 b0)) x0 (toList s4)) ). {
+      assert (StronglySorted ToListProofs.lt (toList s3 ++ ((x, v) :: nil) ++ toList s2)). {
+        eapply sorted_append.
+        + eapply to_List_sorted. eassumption.
+        + simpl. apply SSorted_cons.
+          * eapply to_List_sorted. eassumption.
+          * rewrite Forall_lt. intros. unfold ToListProofs.lt. rewrite <- toList_sem' in H5.
+            destruct (sem s2 x1) eqn : ?.
+            - solve_Bounds e.
+            - inversion H5.
+            - eassumption.
+       + intros. assert (isUB (Some x) y = true). eapply toList_Bounds_UB. apply HB1. apply H5. solve_Bounds e.
+       + intros. simpl in H5. destruct H5.
+          * inversion H5; subst. order e.
+          * assert (isLB (Some x) y = true). eapply toList_Bounds_LB. apply H3_0. apply H5. solve_Bounds e. }
+      eapply fold_right_proper.
+      - simpl. remember (fromDistinctAscList ((toList s3 ++ ((x, v) :: nil) ++ toList s2))) as m.
+        assert (toList m ==  (toList s3 ++ ((x, v) :: nil) ++ toList s2) = true). { rewrite Heqm.
+        eapply fromDistinctAscList_toList. apply H5. }
+        rewrite <- eq_list_equiv. eapply Eq_Transitive. apply Eq_Symmetric. apply H7.
+        unfold is_true. rewrite <-eq_toList. eapply strong_eq1.
+        + subst. eapply fromDistinctAscList_Desc. apply H5. intros. apply H8.
+        + wf_bounds.
+        + intros. rewrite Hsem1. rewrite Heqm. eapply fromDistinctAscList_Desc. apply H5. intros.
+          rewrite H10. simpl. rewrite sem_list_app.
+          destruct (i0 > i) eqn : ?.
+          * erewrite <- toList_sem''. simpl. unfold SomeIf.  erewrite <- toList_sem''.
+            rewrite Hsem. rewrite Heqb0. 
+            destruct (sem s1 i0).
+            -- reflexivity.
+            -- destruct (i0 == x); reflexivity.
+            -- eassumption.
+            -- eassumption.
+          * erewrite <- toList_sem''. rewrite Hsem. rewrite Heqb0. simpl.
+            -- destruct (i0 == x) eqn : ?.
+                ++ solve_Bounds e.
+                ++ erewrite <- toList_sem''. eapply sem_outside_below. eassumption. solve_Bounds e.
+                   eassumption.
+            -- eassumption.
+        + rewrite Heqm. apply fromDistinctAscList_Desc. apply H5. intros. apply H8.
+        + wf_bounds.
+      - intros. apply H2 in H7. destruct p1. destruct p2. 
+        eapply equal_f in H7. rewrite H7. reflexivity. }
+    rewrite H5. reflexivity. apply HB2. apply H3_0. apply HB1.
+    + repeat(applyDesc e (@map_gt_Desc e a)). repeat (erewrite mapAccumRWithKey_fst).
+      * assert (forall i, sem s2 i = sem s3 i). {
+         intros. destruct (_GHC.Base.>_ i0 i) eqn : ?.
+          - specialize (Hsem i0). rewrite Heqb1 in Hsem. simpl in Hsem.
+            rewrite Hsem. assert (sem s1 i0 = None). eapply sem_outside_above. eassumption.
+            solve_Bounds e. rewrite H7. simpl. assert (i0 == x = false) by (order e). rewrite H8.
+            reflexivity.
+          - specialize (Hsem i0).  rewrite Hsem. rewrite Heqb1. eapply sem_outside_below. eassumption.
+            solve_Bounds e. } 
+        assert ((foldrWithKey (fun  (k : e) (v0 : a) (t : b) => fst (f t k v0)) x0 s2) =
+           (foldrWithKey (fun (k : e) (v0 : a) (t : b)  => fst (f t k v0)) x0 s3)). {
+            eapply foldRWithKey_equiv_maps. wf_bounds. wf_bounds. intros.
+            assert (f y e1 a1 = f y e2 a2). { unfold respectful in H2. unfold Proper in H2.
+            remember (e1, a1). remember (e2, a2). assert (p == p0 = true). unfold_pair.
+            subst. rewrite andb_true_iff. split; assumption. apply H2 in H10. subst.
+            eapply equal_f in H10. apply H10. } rewrite H10. reflexivity.
+            intros. rewrite H7. reflexivity. }
+        rewrite H8.
+        assert (forall z,  f z x v = f z i v).  { intros.
+        remember (x,v). remember (i,v). assert (p == p0 = true). unfold_pair. subst.
+        rewrite andb_true_iff. split. order e. order a. apply H2 in H9. subst. eapply equal_f in H9.
+        apply H9. } rewrite H9. reflexivity.
+      * eassumption.
+      * eassumption.
+    + repeat(applyDesc e (@map_gt_Desc e a)). repeat (erewrite mapAccumRWithKey_fst).
+      * assert (forall i, sem s4 i = sem s3 i). {
+        intros.  destruct (_GHC.Base.>_ i0 i) eqn : ?.
+        - rewrite Hsem. rewrite Hsem0. simpl. rewrite Heqb1. assert (sem s1 i0 = None). eapply sem_outside_above.
+          eassumption. solve_Bounds e. rewrite H5. simpl. 
+          assert (i0 == x = false) by (solve_Bounds e). rewrite H7. reflexivity.
+        - rewrite Hsem0. rewrite Hsem. rewrite Heqb1. reflexivity. }
+        assert ((foldrWithKey (fun (k : e) (v0 : a)(t : b)  => fst (f t k v0)) x0 s3) =
+           (foldrWithKey (fun (k : e) (v0 : a)(t : b)  => fst (f t k v0)) x0 s4)). {
+          eapply foldRWithKey_equiv_maps. wf_bounds. wf_bounds. intros.
+          assert (f y e1 a1 = f y e2 a2). { unfold respectful in H2. unfold Proper in H2.
+          remember (e1, a1). remember (e2, a2). assert (p == p0 = true). unfold_pair.
+          subst. rewrite andb_true_iff. split; assumption. apply H2 in H9. subst.
+          eapply equal_f in H9. apply H9. } rewrite H9. reflexivity. 
+          intros. rewrite H5. reflexivity. }
+      rewrite H7. reflexivity. 
+     * eassumption.
+     * eassumption.
+    
+Qed. 
+
+(** Vertification of [mapKeys] *)
+
+(*Note: only have None because we do not know the bounds given by fromList*)
+(*This is a bit of a lazy specification, but it says that the keys values can be found by looking
+  backwards in the list produced by folding the function over the keys*)
+Lemma mapKeys_Desc: forall {e e' a} `{OrdLaws e} `{OrdLaws e'} (f: e -> e') (m: Map e a) ub lb,
+  Bounded m lb ub ->
+  Desc' (mapKeys f m) None None 
+  (fun i => sem_for_lists (rev (foldrWithKey (fun k v t => ((f k), v) :: t) nil m)) i).
+Proof.
+  intros. unfold mapKeys. eapply (@fromList_Desc e' a). apply H0.
+Qed.
+
+(*[mapKeysWith] requires fromListWith, so it is not done yet*)
+  
+(** Verification of [mapKeysMonotonic] *)
+
+Definition f_bound {e e'} (f: e -> e') (b: bound) : bound :=
+  match b with
+  |None => None
+  |Some y => Some (f y)
+  end.
+
+Lemma fold_right_map: forall {a b} (l: list a) (f : a -> b),
+  fold_right (fun x t => (f x) :: t) nil l = List.map (fun x => f x) l.
+Proof.
+  intros. induction l.
+  - simpl. reflexivity.
+  - simpl. rewrite IHl. reflexivity.
+Qed.
+
+Lemma fold_right_scope: forall {e e' a} (l: list (e * a)) (f : e -> e'),
+    fold_right (fun (x0 : e * a) (t : list (e' * a)) => let (a0, b) := x0 in (f a0, b) :: t) nil l =
+    fold_right (fun (x0 : e * a) (t : list (e' * a)) => (let (a0, b) := x0 in (f a0, b)) :: t) nil l.
+Proof.
+  intros. induction l.
+  - reflexivity.
+  - simpl. destruct a0. rewrite IHl. reflexivity.
+Qed. 
+
+(*Here we can give actual bounds and do not need to reverse the resulting list. The proof is a bit longer
+  because the function is not defined using fromList*)
+Lemma mapKeysMonotonic_Desc: forall {e e' a} `{OrdLaws e} `{OrdLaws e'} (f: e -> e') (m : Map e a) lb ub,
+  Bounded m lb ub ->
+  (forall x y, x < y = true -> (f x < f y) = true) ->
+  Desc (mapKeysMonotonic f m) (f_bound f lb) (f_bound f ub) (size m) 
+  (fun i => sem_for_lists(foldrWithKey (fun k v t => ((f k), v) :: t) nil m) i).
+Proof.
+  intros. induction H1.
+  - simpl. solve_Desc e.
+  - simpl. applyDesc e IHBounded1. applyDesc e IHBounded2. solve_Desc e. 
+    + destruct lb. assert (e0 < x = true) by (solve_Bounds e). simpl. apply H2. apply H6. reflexivity.
+    + destruct ub. assert (x < e0 = true) by (solve_Bounds e). simpl. apply H2. apply H6. reflexivity.
+    + intros. repeat (erewrite foldrWithKey_spec'). 
+    assert (fold_right (fun (x0 : e * a) (t : list (e' * a)) => let (a0, b) := x0 in (f a0, b) :: t)
+     ((f x, v)
+      :: fold_right (fun (x0 : e * a) (t : list (e' * a)) => let (a0, b) := x0 in (f a0, b) :: t) nil (toList s2))
+     (toList s1) = 
+      fold_right (fun (x0 : e * a) (t : list (e' * a)) => let (a0, b) := x0 in (f a0, b) :: t) 
+       nil (toList s1 ++ (x, v) :: toList s2)). { rewrite fold_right_app. simpl. reflexivity. }
+    rewrite H6. clear H6. 
+    assert ((fold_right (fun (x0 : e * a) (t : list (e' * a)) => let (a0, b) := x0 in (f a0, b) :: t) nil
+     (toList s1 ++ (x, v) :: toList s2)) = List.map (fun (x0 : e * a) => let (x, y) := x0 in (f x, y))
+    (toList s1 ++ (x, v) :: toList s2)). { 
+    rewrite <- (fold_right_map (toList s1 ++ (x, v) :: toList s2) (fun x => let (a, b) := x in (f a, b))).
+    rewrite fold_right_scope. reflexivity. }
+    rewrite H6. rewrite map_app. simpl. rewrite sem_list_app. simpl.
+    repeat(rewrite <- fold_right_map). repeat(rewrite <- fold_right_scope). repeat(rewrite <- foldrWithKey_spec').
+    rewrite <- Hsem. rewrite <- Hsem0. destruct (sem s i). reflexivity. destruct (i == (f x)); reflexivity.
+Qed.
+
