examples/containers/theories/MapProofs/PairTypeclass.v
@@ -1,0 +1,127 @@
+Require Import GHC.Base.
+Import GHC.Base.Notations.
+Require Import Proofs.GHC.Base.
+Require Import Data.Map.Internal.
+Import GHC.Num.Notations.
+Require Import OrdTactic.
+Require Import Psatz.
+Require Import Tactics.
+Set Bullet Behavior "Strict Subproofs".
+
+Lemma Eq_Tuple_Trans: forall {e a} `{EqLaws e} `{EqLaws a} (x1 x2 x3 : e) (y1 y2 y3 : a),
+  (x1, y1) == (x2, y2) = true -> (x2, y2) == (x3, y3) = true -> (x1, y1) == (x3, y3) = true.
+Proof.
+  intros. unfold op_zeze__ in *. unfold Eq_pair___ in *. unfold op_zeze____ in *. unfold eq_pair in *.
+  rewrite andb_true_iff in *. destruct H3. destruct H4. split. eapply Eq_Transitive. apply H3. apply H4.
+  eapply Eq_Transitive. apply H5. apply H6.
+Qed.
+
+Lemma Eq_Tuple_Sym: forall {e a} `{EqLaws e} `{EqLaws a} (x1 x2 : e) (y1 y2 : a),
+  (x1, y1) == (x2, y2) = true <-> (x2, y2) == (x1, y1) = true.
+Proof.
+  intros. unfold op_zeze__ in *. unfold Eq_pair___  in *. unfold op_zeze____ in *. unfold eq_pair in *.
+  rewrite andb_true_iff in *. rewrite andb_true_iff in *. split; intros.
+  - destruct H3. split. apply Eq_Symmetric. apply H3. apply Eq_Symmetric. apply H4.
+  - destruct H3. split. apply Eq_Symmetric. apply H3. apply Eq_Symmetric. apply H4.
+Qed. 
+
+Lemma Eq_Tuple_Refl: forall {e a} `{EqLaws e} `{EqLaws a} (x :e) (y : a),
+  (x, y) == (x, y) = true.
+Proof.
+  intros. unfold_zeze. unfold eq_pair. rewrite andb_true_iff. split; apply Eq_Reflexive.
+Qed.
+
+Lemma eq_tuple_prop: forall {a} {b} `{Eq_ a} `{EqLaws a} `{Eq_ b} `{EqLaws b}
+  (x1 x2 : a) (y1 y2 : b),
+  (x1, y1) == (x2, y2) = true <-> x1 == x2 = true /\ y1 == y2 = true.
+Proof.
+  intros. unfold op_zeze__. unfold Eq_pair___. unfold op_zeze____. unfold eq_pair.
+  unfold op_zeze__. unfold op_zeze____. rewrite andb_true_iff. reflexivity.
+Qed.
+
+Lemma prop_bool: forall (b1: bool) (b2: bool),
+  b1 = b2 <-> (b1 = true <-> b2 = true).
+Proof.
+  intros. split; intros.
+  - split; intros.
+    + subst. reflexivity.
+    + subst. reflexivity.
+  - destruct H. destruct b1. symmetry. apply H. reflexivity.
+    destruct b2. apply H0. reflexivity. reflexivity.
+Qed.
+
+Lemma eq_tuple_eq: forall {a} {b} `{Eq_ a} `{EqLaws a} `{Eq_ b} `{EqLaws b}
+  (x1 x2 : a) (y1 y2 : b),
+  (x1, y1) == (x2, y2) = (x1 == x2) && (y1 == y2).
+Proof. 
+  intros. rewrite prop_bool. rewrite andb_true_iff. apply eq_tuple_prop.
+Qed.
+
+(*First, we need lawful [Eq] and [Ord] instances for pairs*)
+Global Instance EqLaws_Pair {a} {b} `{EqLaws a} `{EqLaws b} : EqLaws (a * b).
+Proof.
+  constructor.
+  - unfold "==". unfold Eq_pair___. unfold op_zeze____. unfold eq_pair. unfold ssrbool.reflexive.
+    intros. destruct x. unfold is_true. rewrite andb_true_iff. split; apply Eq_Reflexive.
+  - unfold "==". unfold Eq_pair___. unfold op_zeze____. unfold eq_pair. unfold ssrbool.symmetric.
+    intros. destruct x. destruct y. assert ((a0 == a1) = (a1 == a0)) by (order a).
+    assert ((b0 == b1) = (b1 == b0)) by (order b). rewrite H3. rewrite H4. reflexivity.
+  - unfold "==". unfold Eq_pair___. unfold op_zeze____. unfold eq_pair. unfold ssrbool.transitive.
+    intros. destruct x. destruct y. destruct z. unfold is_true in *.
+    rewrite andb_true_iff in H3. rewrite andb_true_iff in H4. destruct H3. destruct H4.
+    eapply Eq_Tuple_Trans. rewrite eq_tuple_prop. split. apply H3. apply H5. rewrite eq_tuple_prop.
+    split. apply H4. apply H6.
+  - intros. unfold "==", "/=". unfold Eq_pair___. unfold op_zeze____ , op_zsze____ .
+    destruct (eq_pair x y). reflexivity. reflexivity.
+Qed.
+
+(*If a and b are lawful members of [Ord], then so is a * b*)
+Instance OrdLaws_Pair {a} {b} `{OrdLaws a} `{OrdLaws b} : OrdLaws (a * b).
+Proof.
+  constructor.
+  - intros. destruct a0. destruct b0. unfold "<=", "==" in *. unfold Ord_pair___, Eq_pair___ in *.
+    unfold ord_default, op_zeze____  in *. simpl in *.
+    rewrite andb_true_iff.  rewrite negb_true_iff in *. 
+    destruct (compare a1 a0) eqn : ?. destruct (compare b0 b1) eqn : ?. split. order a. order b.
+    inversion H1. split. order a. assert (compare a0 a1 = Eq) by (order a). rewrite H3 in H2.
+    assert (compare b1 b0 = Lt) by (order b). rewrite H4 in H2. inversion H2. inversion H1.
+    assert (compare a0 a1 = Lt) by (order a). rewrite H3 in H2. inversion H2. 
+  - intros. destruct a0. destruct c. destruct b0. unfold "<=" in *. unfold Ord_pair___  in *.
+    unfold compare_pair in *. unfold ord_default in *. simpl in *. rewrite negb_true_iff in *.
+    repeat (try (destruct (compare a2 a0) eqn : ?); try (destruct (compare a1 a2) eqn : ?);
+    try (destruct (compare b0 b1) eqn : ?); try (destruct (compare b2 b0) eqn : ?);
+    try (destruct (compare a1 a0) eqn : ?); try (destruct (compare b2 b1) eqn : ?); try (order a);
+    try (order b)).
+  - intros. destruct a0. destruct b0. unfold "<=" in *. unfold Ord_pair___ in *. unfold compare_pair in *.
+    unfold ord_default. unfold ord_default in *. simpl. rewrite negb_true_iff. rewrite negb_true_iff.
+    destruct (compare a1 a0) eqn : ?. assert (compare a0 a1 = Eq) by (order a). rewrite H1.
+    destruct (compare b0 b1) eqn : ?. left. reflexivity. right. assert (compare b1 b0 <> Lt) by (order b).
+    destruct (compare b1 b0). reflexivity. contradiction. reflexivity. left. reflexivity.
+    right. destruct (compare a0 a1) eqn : ?. order a. order a. reflexivity.
+    left. reflexivity.
+  - intros. unfold compare.   unfold "<=" in *. unfold Ord_pair___ in *. unfold compare_pair in *.
+    unfold ord_default. simpl. rewrite negb_false_iff. destruct a0. destruct b0. 
+    split; intros. destruct (compare a0 a1). rewrite H1. reflexivity. reflexivity. inversion H1.
+    destruct (compare a0 a1). destruct (compare b1 b0). inversion H1. reflexivity. inversion H1.
+    reflexivity. inversion H1.
+  - intros. unfold compare. unfold "==". unfold Ord_pair___ , Eq_pair___ . unfold compare_pair,op_zeze____ .
+    unfold ord_default, eq_pair. simpl. destruct a0. destruct b0. split; intros. destruct (compare a0 a1) eqn : ?.
+    inversion H. rewrite Ord_compare_Eq in Heqc. inversion H0. rewrite Ord_compare_Eq0 in H1. rewrite andb_true_iff.
+    split; assumption. inversion H1. inversion H1. rewrite andb_true_iff in H1. destruct H1.
+    inversion H. inversion H0. apply Ord_compare_Eq in H1. apply Ord_compare_Eq0 in H2. rewrite H1. assumption.
+  - intros. unfold compare. unfold Ord_pair___ , "<=". unfold compare_pair. unfold ord_default. simpl.
+    destruct a0. destruct b0. split; intros. rewrite negb_false_iff.  
+    destruct (compare a0 a1) eqn : ?. assert (compare a1 a0 = Eq) by (order a). rewrite H2.
+    assert (compare b0 b1 = Lt) by (order b). rewrite H3. reflexivity. inversion H1. inversion H1.
+    assert (compare a1 a0 = Lt) by (order a). rewrite H2. reflexivity.
+    rewrite negb_false_iff in H1. destruct (compare a1 a0) eqn : ?.
+    assert (compare a0 a1 = Eq) by (order a). rewrite H2. destruct (compare b0 b1) eqn : ?.
+    inversion H1. order b. inversion H1. assert (compare a0 a1 = Gt) by (order a). rewrite H2.
+    reflexivity. inversion H1.
+  - intros. unfold "<", "<=". unfold Ord_pair___.  unfold compare_pair; unfold ord_default; simpl.
+    rewrite negb_involutive. reflexivity.
+  - intros. unfold "<=", ">=". unfold Ord_pair___. unfold compare_pair; unfold ord_default; simpl.
+    reflexivity.
+  - intros. unfold ">", "<=". unfold Ord_pair___.  unfold compare_pair; unfold ord_default; simpl.
+    rewrite negb_involutive. reflexivity.
+Qed.
